\documentclass[12pt]{article}
\usepackage{amsmath,amssymb}
\usepackage[utf8x]{inputenc}
\usepackage{amsfonts}
\usepackage[T1]{fontenc}
\usepackage{tikz}
\usepackage{pgf}
\usepackage{xcolor}
\usetikzlibrary{cd}


\begin{document}
\begin{gather*}
\tilde{L}_2=(L_{21},\dots,L_{2n}),\quad
L_{2k}:\mathbb{F}_q^m\to\mathbb{F}_q^m\\
L_{2k}(\underline{y}_k)=\underline{y}_k B_{2k},\quad
B_{2k}=(B_{ij}^k)\in\operatorname{M}_{m\times m}(\mathbb{F}_q),\quad
|B_{2k}|\neq 0
\end{gather*}

\begin{gather*}
L_3=\rho\circ\tilde{L}_3\circ\tilde{\pi}_2,\quad
\tilde{L}_3=(L_{31},\dots,L_{3n}),\\
L_{3k}(\underline{z}_k)=\underline{z}_k C_{3k},\quad
C_{3k}=(C_{ij}^k)\in\operatorname{M}_{n\times n}(\mathbb{F}_q),\quad
|C_{3k}|\neq 0
\end{gather*}

\begin{gather*}
A_1\in\operatorname{M}_{m\times m}(\mathbb{Z}_{q^n-1}),\quad \gcd(|A_1|,q^n-1)=1\\
G_1:(\mathbb{F}_{q^n})^m\to(\mathbb{F}_{q^n})^m,\quad
G_1(u_1,\dots,u_m)=(u_1^{a_{11}}\dots u_m^{a_{1m}},\dots,u_1^{a_{m1}}\dots u_m^{a_{mm}})
\end{gather*}

\begin{gather*}
A_1^{-1}\in\operatorname{M}_{m\times m}(\mathbb{Z}_{q^n-1}),\quad 
(\mathbb{F}_{q^n}\setminus\{0\})^n
\end{gather*}

\begin{gather*}
A_2\in\operatorname{M}_{n\times n}(\mathbb{Z}_{q^m-1}),\quad\gcd(|A_2|,q^m-1)=1\\
G_2:(\mathbb{F}_{q^m})^n\to(\mathbb{F}_{q^m})^n,\quad
G_2(v_1,\dots,v_n)=(v_1^{b_{11}}\dots v_n^{b_{1n}},\dots,v_1^{b_{n1}}\dots v_n^{b_{nn}})
\end{gather*}

\begin{gather*}
F(x_{1},\dots,x_{nm})=(z_{1},\dots,z_{mn}),\quad F_k(\underline{x})\in\mathbb{F}_q[x_{1},\dots,x_{nm}]\\
DM:\mathbb{F}_q^N\to\mathbb{F}_q^{nm}\quad
F^{-1}(\underline{z})=L_1^{-1}\circ G_1^{-1}\circ L_2^{-1}\circ G_2^{-1}\circ L_3^{-1}(\underline{z})
\end{gather*}

\begin{gather*}
\overline{x}_1,\dots,\overline{x}_k\in\mathbb{F}_q^N,\quad
\underline{x}_i=H(\overline{x}_i)\in\mathbb{F}_q^{nm}
\end{gather*}

\begin{gather*}
\underline{z}_i,\quad (\underline{z}_i)_j=F_j(\underline{x}_i)=\sum_u f_{u,j} M_u(\underline{x}_i)
\end{gather*}

\begin{gather*}
\underline{z}=DM(\overline{x}),\quad \underline{z}\in\mathbb{F}_q^{nm}
\end{gather*}

\begin{gather*}
h_1:\{1,\dots,N\}\to\{1,\dots,nm\}\\
s=\operatorname{sig}(\overline{z})=(\overline{z},\overline{x},h_1)\\
\overline{y}=DM_B(\overline{x}),\quad \overline{z}=DM_A^{-1}(\overline{y})
\end{gather*}

\begin{gather*}
HAS:\mathbb{F}_2^e\to\mathbb{F}_2^b,\quad q=2^e\quad b<e\cdot N,\quad w=HAS(x)
\end{gather*}




\end{document}
